theories/lang/mailbox_extra.v
@@ -5,29 +5,31 @@ From HypVeri.algebra Require Import base.
 Section mailbox_extra.
 
 Context {HyperConst : HypervisorConstants}.
+Implicit Type σ : state.
+Implicit Type i : VMID.
 
 Lemma empty_rx_global_preserve_current_vm σ i :
-  (get_current_vm (empty_rx_global σ i)) = (get_current_vm σ).
+  get_current_vm (empty_rx_global σ i) = get_current_vm σ.
 Proof.
   rewrite /empty_rx_global.
-  rewrite (surjective_pairing (get_vm_mail_box σ i)).
-  by rewrite (surjective_pairing (get_vm_mail_box σ i).2).
+  rewrite (surjective_pairing (get_mail_box σ @ i)).
+  by rewrite (surjective_pairing (get_mail_box σ @ i).2).
 Qed.
 
 Lemma empty_rx_global_preserve_mem σ i :
   get_mem (empty_rx_global σ i) = get_mem σ.
 Proof.
   rewrite /empty_rx_global.
-  rewrite (surjective_pairing (get_vm_mail_box σ i)).
-  by rewrite (surjective_pairing (get_vm_mail_box σ i).2).
+  rewrite (surjective_pairing (get_mail_box σ @ i)).
+  by rewrite (surjective_pairing (get_mail_box σ @ i).2).
 Qed.
 
 Lemma empty_rx_global_preserve_regs σ i :
  get_reg_gmap (empty_rx_global σ i) = get_reg_gmap σ.
 Proof.
   rewrite /empty_rx_global.
-  rewrite (surjective_pairing (get_vm_mail_box σ i)).
-  by rewrite (surjective_pairing (get_vm_mail_box σ i).2).
+  rewrite (surjective_pairing (get_mail_box σ @ i)).
+  by rewrite (surjective_pairing (get_mail_box σ @ i).2).
 Qed.
 
 (* TODO *)
@@ -35,9 +37,9 @@ Lemma empty_rx_global_preserve_mb σ i :
   get_mb_gmap (empty_rx_global σ i) = (get_mb_gmap σ).
 Proof.
   rewrite /empty_rx_global.
-  rewrite (surjective_pairing (get_vm_mail_box σ i)).
-  rewrite (surjective_pairing (get_vm_mail_box σ i).2).
-  rewrite /get_mb_gmap /get_vm_mail_box /get_mail_boxes /=.
+  rewrite (surjective_pairing (get_mail_box σ @ i)).
+  rewrite (surjective_pairing (get_mail_box σ @ i).2).
+  rewrite /get_mb_gmap /=.
   f_equal.
   (* apply (list_eq_same_length _ _ (2*vm_count)). *)
   (* induction list_of_vmids eqn:Heqn. *)
@@ -74,56 +76,56 @@ Lemma empty_rx_global_preserve_pagetable σ i:
   get_page_table (empty_rx_global σ i)  = get_page_table σ.
 Proof.
   rewrite /empty_rx_global.
-  rewrite (surjective_pairing (get_vm_mail_box σ i)).
-  by rewrite (surjective_pairing (get_vm_mail_box σ i).2).
+  rewrite (surjective_pairing (get_mail_box σ @ i)).
+  by rewrite (surjective_pairing (get_mail_box σ @ i).2).
 Qed.
 
 Lemma empty_rx_global_preserve_owned σ i :
   get_owned_gmap (empty_rx_global σ i) = (get_owned_gmap σ).
 Proof.
   rewrite /empty_rx_global.
-  rewrite (surjective_pairing (get_vm_mail_box σ i)).
-  by rewrite (surjective_pairing (get_vm_mail_box σ i).2).
+  rewrite (surjective_pairing (get_mail_box σ @ i)).
+  by rewrite (surjective_pairing (get_mail_box σ @ i).2).
 Qed.
 
 Lemma empty_rx_global_preserve_access σ i :
   get_access_gmap (empty_rx_global σ i) = (get_access_gmap σ).
 Proof.
   rewrite /empty_rx_global.
-  rewrite (surjective_pairing (get_vm_mail_box σ i)).
-  by rewrite (surjective_pairing (get_vm_mail_box σ i).2).
+  rewrite (surjective_pairing (get_mail_box σ @ i)).
+  by rewrite (surjective_pairing (get_mail_box σ @ i).2).
 Qed.
 
 Lemma empty_rx_global_preserve_trans σ i :
   get_trans_gmap (empty_rx_global σ i) = (get_trans_gmap σ).
 Proof.
   rewrite /empty_rx_global.
-  rewrite (surjective_pairing (get_vm_mail_box σ i)).
-  by rewrite (surjective_pairing (get_vm_mail_box σ i).2).
+  rewrite (surjective_pairing (get_mail_box σ @ i)).
+  by rewrite (surjective_pairing (get_mail_box σ @ i).2).
 Qed.
 
 Lemma empty_rx_global_preserve_trans' σ i :
   get_transactions (empty_rx_global σ i) = (get_transactions σ).
 Proof.
   rewrite /empty_rx_global.
-  rewrite (surjective_pairing (get_vm_mail_box σ i)).
-  by rewrite (surjective_pairing (get_vm_mail_box σ i).2).
+  rewrite (surjective_pairing (get_mail_box σ @ i)).
+  by rewrite (surjective_pairing (get_mail_box σ @ i).2).
 Qed.
 
 Lemma empty_rx_global_preserve_hpool σ i :
   get_hpool_gset (empty_rx_global σ i) = (get_hpool_gset σ).
 Proof.
   rewrite /empty_rx_global.
-  rewrite (surjective_pairing (get_vm_mail_box σ i)).
-  by rewrite (surjective_pairing (get_vm_mail_box σ i).2).
+  rewrite (surjective_pairing (get_mail_box σ @ i)).
+  by rewrite (surjective_pairing (get_mail_box σ @ i).2).
 Qed.
 
 Lemma empty_rx_global_preserve_retri σ i :
   get_retri_gmap (empty_rx_global σ i) = (get_retri_gmap σ).
 Proof.
   rewrite /empty_rx_global.
-  rewrite (surjective_pairing (get_vm_mail_box σ i)).
-  by rewrite (surjective_pairing (get_vm_mail_box σ i).2).
+  rewrite (surjective_pairing (get_mail_box σ @ i)).
+  by rewrite (surjective_pairing (get_mail_box σ @ i).2).
 Qed.
 
 
@@ -135,23 +137,20 @@ Proof.
   apply map_eq.
   intros i.
   destruct (list_to_map
-              (map
-                 (λ v0 : VMID,
-                         match (get_vm_mail_box (empty_rx_global σ l) v0).2.2 with
-                         | Some (l0, j) => (v0, Some (l0, j))
-                         | None => (v0, None)
-                         end
-                 )
-                 list_of_vmids) !! i) eqn:Heqn.
+    (map
+       (λ v : fin vm_count,
+          match get_transactions (get_transactions get_mail_boxes empty_rx_global σ l !!! v) with
+          | Some (l0, j) => (v, Some (l0, j))
+          | None => (v, None)
+          end) list_of_vmids) !! i) eqn:Heqn.
   - apply elem_of_list_to_map_2 in Heqn.
     apply elem_of_list_In in Heqn.
     apply in_map_iff in Heqn.
     destruct Heqn as [y [Heqn1 Heqn2]].
     apply elem_of_list_In in Heqn2.
     rewrite /empty_rx_global //= in Heqn1.
-    rewrite (surjective_pairing (get_vm_mail_box σ l)) in Heqn1.
-    rewrite (surjective_pairing (get_vm_mail_box σ l).2) in Heqn1.
-    rewrite /get_vm_mail_box /get_mail_boxes in Heqn1.
+    rewrite (surjective_pairing (get_mail_box σ @ l)) in Heqn1.
+    rewrite (surjective_pairing (get_mail_box σ @ l).2) in Heqn1.
     simpl in Heqn1.
     destruct (decide (l = y)).
     + subst.
@@ -162,7 +161,6 @@ Proof.
       reflexivity.
     + symmetry.
       rewrite lookup_insert_Some.
-      rewrite /get_vm_mail_box /get_mail_boxes //= in Heqn1.
       rewrite vlookup_insert_ne in Heqn1; auto.
       destruct (σ.1.1.1.1.2 !!! y) as [a b] eqn:Heqn3.
       destruct b as [c d] eqn:Heqn4.
@@ -170,7 +168,6 @@ Proof.
       destruct d as [e|] eqn:Heqn5.
       * destruct e as [f g] eqn:Heqn6.
         inversion Heqn1; subst; clear Heqn1.
-        rewrite /get_vm_mail_box /get_mail_boxes.
         right.
         split; auto.
         apply elem_of_list_to_map_1'.
@@ -196,7 +193,6 @@ Proof.
            apply elem_of_list_In in Heqn2.
            split; auto.
       * simplify_eq.
-        rewrite /get_vm_mail_box /get_mail_boxes //=.
         right.
         split; auto.
         apply elem_of_list_to_map_1'.
@@ -224,9 +220,8 @@ Proof.
   - symmetry.
     rewrite <-not_elem_of_list_to_map in Heqn.
     rewrite /empty_rx_global //= in Heqn.
-    rewrite (surjective_pairing (get_vm_mail_box σ l)) in Heqn.
-    rewrite (surjective_pairing (get_vm_mail_box σ l).2) in Heqn.
-    rewrite /get_vm_mail_box /get_mail_boxes in Heqn.
+    rewrite (surjective_pairing (get_mail_box σ @ l)) in Heqn.
+    rewrite (surjective_pairing (get_mail_box σ @ l).2) in Heqn.
     simpl in Heqn.
     destruct (decide (l = i)).
     + subst.
@@ -234,17 +229,17 @@ Proof.
       apply Heqn.
       rewrite <-list_fmap_compose.
       rewrite /compose.
-      rewrite /get_vm_mail_box /fill_rx_unsafe /get_mail_boxes //=.
+      rewrite /fill_rx_unsafe //=.
       apply elem_of_list_In.
       apply in_map_iff.
       exists i.
       split; auto using in_list_of_vmids.
       rewrite vlookup_insert //=.
-    + rewrite /get_vm_mail_box /fill_rx_unsafe /get_mail_boxes //=.
+    + rewrite /fill_rx_unsafe //=.
       rewrite lookup_insert_None.
       split; auto.
       rewrite <-not_elem_of_list_to_map.
-      rewrite /get_vm_mail_box /fill_rx_unsafe /get_mail_boxes //= in Heqn.
+      rewrite /fill_rx_unsafe //= in Heqn.
       intros H.
       apply Heqn.
       apply elem_of_list_In.
